Regex/Compiler/Lemmas/Basic.lean
@@ -1,0 +1,238 @@
+
+import Std.Tactic.Do
+import Std.Tactic.Do.Syntax
+
+import Regex.Compiler.Basic
+import Regex.Compiler.Compile
+
+namespace Compiler
+
+open Syntax
+open NFA
+
+namespace Lemmas
+
+/-- instantiate mvar,
+    mspec with a precondition like `fun s => s = states ∧ P` gives a uninstantiated mvar
+-/
+syntax "inst_mvar" : tactic
+macro_rules | `(tactic|inst_mvar) => `(tactic| simp; (try and_intros; rfl); try simp_all)
+
+/-- instantiate mvars,
+    mspec with a precondition like `fun s => s = states ∧ P` gives a uninstantiated mvar
+-/
+syntax "inst_mvars" : tactic
+macro_rules | `(tactic|inst_mvars) => `(tactic| simp; and_intros; all_goals try rfl)
+
+@[simp, grind] def isAppend (s1 s2 : Array Unchecked.State) :=
+  ∃ s', s2 = s1 ++ s'
+
+@[simp, grind .] theorem isAppend_trans (h1 : isAppend s1 s2) (h2 : isAppend s2 s3)
+    : isAppend s1 s3 := by
+  grind
+
+@[grind .] private theorem all_push {sid : Unchecked.State} (states : Array Unchecked.State)
+  (h : Unchecked.State.nextOf sid ≤ states.size)
+  (hlt : ∀ (i : Nat) _, states[i].nextOf < states.size)
+    : ∀ (i : Nat) _, ((states.push sid)[i].nextOf < (states.push sid).size) := by
+  intro i hi
+  have := @Array.getElem_push _ states sid i hi
+  simp_all
+  split
+  . rename_i h'
+    exact Nat.lt_add_right 1 (hlt i h')
+  . exact Nat.lt_add_one_of_le h
+
+open Std.Do
+
+set_option mvcgen.warning false
+
+@[spec] theorem lift_StackT_to_EStateM_spec
+  (v : StateT σ Id α)
+  {P : σ → Prop}
+  (Q : σ → α → σ → Prop)
+  (hspec : ⦃fun s => ⌜s = n ∧ P n⌝⦄ v ⦃post⟨fun a s => ⌜Q n a s⌝⟩⦄)
+    : ⦃fun s => ⌜s = n ∧ P n⌝⦄
+      (v : (EStateM ε σ α))
+      ⦃post⟨fun a s => ⌜Q n a s⌝, fun _ => ⌜False⌝ ⟩⦄ := by
+  assumption
+
+def coe_spec_StackT_to_EStateM
+  {v : StateT σ Id α}
+  {P : σ → Prop}
+  {Q : α → σ → Prop}
+  (hspec : ⦃fun s => ⌜P s⌝⦄ v ⦃post⟨fun a s => ⌜Q a s⌝⟩⦄)
+    : ⦃fun s => ⌜P s⌝⦄
+      (v : (EStateM ε σ α))
+      ⦃post⟨fun a s => ⌜Q a s⌝, fun _ _ => ⌜False⌝ ⟩⦄ := by
+  assumption
+
+instance {v : StateT σ Id α} {P : σ → Prop} {Q : α → σ → Prop}
+  : Coe (⦃fun s => ⌜P s⌝⦄ v ⦃post⟨fun a s => ⌜Q a s⌝⟩⦄)
+      (⦃fun s => ⌜P s⌝⦄ (v : (EStateM ε σ α)) ⦃post⟨fun a s => ⌜Q a s⌝, fun _ _ => ⌜False⌝ ⟩⦄)
+  where coe := coe_spec_StackT_to_EStateM
+
+@[simp, grind] def tRefLt (t : ThompsonRef) (r : Array Unchecked.State) :=
+  t.1 < r.size ∧ t.2 < r.size
+
+@[simp, grind] def statesNextOfLeLt (prevs : Array Unchecked.State) (s : Array Unchecked.State) :=
+  prevs.size ≤ s.size ∧ NextOfLt s
+
+@[simp, grind] def stateIdNextOfLt (prevs : Array Unchecked.State) (sid : Unchecked.StateID) (s : Array Unchecked.State) :=
+  prevs.size < s.size ∧ sid < s.size ∧ NextOfLt s
+
+@[simp, grind] def stateIdNextOfLeLt (prevs : Array Unchecked.State) (sid : Unchecked.StateID) (s : Array Unchecked.State) :=
+  prevs.size ≤ s.size ∧ sid < s.size ∧ NextOfLt s
+
+@[simp, grind] def stateIdNextOfEqLt (prevs : Array Unchecked.State) (sid : Unchecked.StateID) (s : Array Unchecked.State) :=
+  prevs.size = s.size ∧ sid < s.size ∧ NextOfLt s
+
+@[simp, grind] def tRefNextOfLt (prevs : Array Unchecked.State) (t : ThompsonRef) (s : Array Unchecked.State) :=
+  prevs.size < s.size ∧ tRefLt t s ∧ NextOfLt s
+
+@[simp, grind] def tRefNextOfLeLt (prevs : Array Unchecked.State) (t : ThompsonRef) (s : Array Unchecked.State) :=
+  prevs.size ≤ s.size ∧ tRefLt t s ∧ NextOfLt s
+
+def cValid (caps : Array NFA.Capture) :=
+  NFA.Capture.Valid caps
+
+def cMemAndValid (prev caps : Array NFA.Capture) :=
+  (∀ a ∈ prev, a ∈ caps) ∧ NFA.Capture.Valid caps
+
+def cValidFunc (captures : Array NFA.Capture) : Array NFA.Capture → Prop :=
+    fun (curr : Array NFA.Capture) => curr = captures ∧ cValid captures
+
+def cMemAndValidFunc (captures : Array NFA.Capture) : Array NFA.Capture → Prop :=
+    fun (curr : Array NFA.Capture) => curr = captures ∧ cMemAndValid captures curr
+
+@[grind .] theorem cap_exists_of_cap_role_end_of_cValid (caps : Array NFA.Capture) (h : cValid caps)
+  (a : NFA.Capture)  (h1 : a ∈ caps) (h2 : a.role = Capture.Role.End)
+    : ∃ (a' : NFA.Capture), a' ∈ caps ∧ a'.role = Capture.Role.Start ∧ a.group = a'.group := by
+  dsimp only [cValid] at h
+  have := Capture.Valid.forall h
+  simp_all
+
+@[grind .] theorem cValid_of_empty (captures : Array NFA.Capture) (h : captures.size = 0)
+    : cValid captures := by
+  dsimp only [cValid]
+  grind
+
+@[grind .] theorem cValid_of_cMemAndValid (prevs caps : Array NFA.Capture)
+  (h : cMemAndValid prevs caps)
+    : cValid caps := by
+  dsimp [cMemAndValid] at h
+  grind [= cValid]
+
+@[simp] theorem cMemAndValid_of_cValid_of_eq (captures : Array NFA.Capture)
+    : ∀ (s : Array NFA.Capture), s = captures ∧ cValid captures → cMemAndValid captures s := by
+  intro s h
+  unfold cValid at h
+  unfold cMemAndValid
+  rw [h.left]
+  simp_all
+
+@[simp] theorem cMemAndValid_of_push_of_role_start (captures : Array NFA.Capture)
+  (capture : NFA.Capture) (hr : capture.role = Capture.Role.Start) (hc : cValid captures)
+    : cMemAndValid captures (captures.push capture) := by
+  simp [cMemAndValid]
+  simp [cValid] at hc
+  and_intros
+  · grind
+  · apply Capture.Valid.mk
+    intro c
+    have ⟨c', _⟩ := Capture.Valid.forall hc ⟨c, by grind⟩
+    exact ⟨c', by grind⟩
+
+@[grind .] theorem cMemAndValid_of_push_of_role_end (captures : Array NFA.Capture)
+  (capture : NFA.Capture) (hc : cValid captures)
+  (h : ∃ c ∈ captures, c.role = Capture.Role.Start ∧ c.group = capture.group)
+    : cMemAndValid captures (captures.push capture) := by
+  simp [cMemAndValid]
+  simp [cValid] at hc
+  and_intros
+  · grind
+  · apply Capture.Valid.mk
+    intro c
+    cases Array.mem_or_eq_of_mem_push c.property.left
+    · have ⟨c', _⟩ := Capture.Valid.forall hc ⟨c, by grind⟩
+      exact ⟨c', by grind⟩
+    · have ⟨c', _⟩ := h
+      exact ⟨c', by grind⟩
+
+@[simp] theorem cMemAndValidFunc_of_cValidFunc (captures : Array NFA.Capture)
+    : ∀ (s : Array NFA.Capture), cValidFunc captures s → cMemAndValidFunc captures s := by
+  intro s h
+  simp [cValidFunc] at h
+  dsimp only [cMemAndValidFunc]
+  simp_all
+
+theorem coe_spec_EStateM_to_EStateM_Prod
+  (σ₃ : Type)
+  {v₁ : EStateM ε σ₁ α}
+  {P₁ : σ₁ → Prop}
+  {Q₁  : α → σ₁ → Prop}
+  (hspec₁ : ⦃fun s => ⌜P₁ s⌝⦄ v₁ ⦃post⟨fun a s => ⌜Q₁ a s⌝, fun _ => ⌜False⌝⟩⦄)
+  (P₂ : σ₂ → Prop)
+  (Q₂ : σ₂ → Prop)
+  (hpq : ∀ s : σ₂, P₂ s → Q₂ s)
+    : ⦃fun s => ⌜P₁ s.1 ∧ P₂ s.2.1⌝⦄
+      (v₁ : EStateM ε (σ₁ × σ₂ × σ₃) α)
+      ⦃post⟨fun r s => ⌜Q₁ r s.1 ∧ Q₂ s.2.1⌝, fun _ _ => ⌜False⌝ ⟩⦄ := by
+  simp_all [Triple, wp, liftM, monadLift, SPred.entails, EStateM.run]
+  grind
+
+theorem coe_spec_EStateM_to_CompilerM
+  {captures : Array NFA.Capture}
+  {v₁ : EStateM ε σ₁ α}
+  {P₁ : σ₁ → Prop}
+  {Q₁  : α → σ₁ → Prop}
+  (hspec₁ : ⦃fun s => ⌜P₁ s⌝⦄ v₁ ⦃post⟨fun a s => ⌜Q₁ a s⌝, fun _ => ⌜False⌝⟩⦄)
+    : ⦃fun s => ⌜P₁ s.1 ∧ s.2.1 = captures ∧ cValid captures⌝⦄
+      (v₁ : EStateM ε (σ₁ × (Array NFA.Capture) × (Array Nat)) α)
+      ⦃post⟨fun r s => ⌜Q₁ r s.1 ∧ s.2.1 = captures ∧ cMemAndValid captures s.2.1⌝, fun _ _ => ⌜False⌝ ⟩⦄ := by
+  exact coe_spec_EStateM_to_EStateM_Prod (Array Nat) hspec₁
+          (cValidFunc captures) (cMemAndValidFunc captures) (by simp_all)
+
+theorem coe_spec_StateT_to_CompilerM
+  {captures : Array NFA.Capture}
+  {v : StateT σ₁ Id α}
+  {P₁: σ₁ → Prop}
+  {Q₁ : α → σ₁ → Prop}
+  (hspec : ⦃fun s => ⌜P₁ s⌝⦄ v ⦃post⟨fun a s => ⌜Q₁ a s⌝⟩⦄)
+    : ⦃fun s => ⌜P₁ s.1 ∧ s.2.1 = captures ∧ cValid captures⌝⦄
+      (v : EStateM ε (σ₁ × (Array NFA.Capture) × (Array Nat)) α)
+      ⦃post⟨fun r s => ⌜Q₁ r s.1 ∧ s.2.1 = captures ∧ cMemAndValid captures s.2.1⌝, fun _ _ => ⌜False⌝⟩⦄ :=
+  coe_spec_EStateM_to_EStateM_Prod (Array Nat) (coe_spec_StackT_to_EStateM hspec)
+          (cValidFunc captures) (cMemAndValidFunc captures) (by simp_all)
+
+theorem lift_CompilerM_bind_pure [MonadLiftT (EStateM ε σ) Code.CompilerM] (x : EStateM ε σ α)
+    : liftM x >>= EStateM.pure = (x : Code.CompilerM α) := by
+  apply bind_pure
+
+theorem pure_of_imp_spec {x : α} {P1 P2 : α → σ → Prop} (h : ∀ a s, P1 a s → P2 a s)
+    : ⦃fun s => ⌜P1 x s⌝⦄
+      (EStateM.pure x : EStateM ε σ α)
+      ⦃post⟨fun r s => ⌜P2 r s⌝, fun _ => ⌜False⌝⟩⦄ := by
+  simp [Triple, wp, EStateM.pure]
+  grind
+
+@[grind .] theorem nextOf_look_eq : (Unchecked.State.Look look 0).nextOf = 0 := by
+  simp_all [Unchecked.State.nextOf]
+
+@[grind .] theorem nextOf_union_eq : (Unchecked.State.Union #[]).nextOf = 0 := by
+  simp_all [Unchecked.State.nextOf, List.maxD]
+
+@[grind .] theorem nextOf_union_reverse_eq : (Unchecked.State.UnionReverse #[]).nextOf = 0 := by
+  simp_all [Unchecked.State.nextOf, List.maxD]
+
+@[grind .] theorem nextOf_transition_le_of_le (states: Array Unchecked.State) (trans : Array Unchecked.Transition)
+  (h : ∀ (i : Nat) (x : i < trans.size), trans[i].next ≤ states.size)
+    : (Unchecked.State.SparseTransitions trans).nextOf ≤ states.size := by
+  simp_all [Unchecked.State.nextOf]
+  have h : ∀ a ∈ trans.toList, a.next ≤ states.size := by
+    intro a ha
+    have ha : a ∈ trans := Array.mem_def.mpr ha
+    have ⟨i, ⟨hlt, heq⟩⟩ := Array.mem_iff_getElem.mp ha
+    have := h i hlt
+    simp_all
+  exact List.maxD_of_all_map_le h
