Regex/Compiler/Lemmas/Compile.lean
@@ -1,0 +1,615 @@
+import Std.Tactic.Do
+import Std.Tactic.Do.Syntax
+
+import Regex.Compiler.Basic
+import Regex.Compiler.Patch
+import Regex.Compiler.Compile
+import Regex.Compiler.Lemmas.Basic
+import Regex.Compiler.Lemmas.Patch
+import Regex.Compiler.Lemmas.AddState
+
+namespace Compiler
+
+open Syntax
+open NFA
+
+namespace Lemmas
+
+/-!
+## Lemmas
+
+Proof that `Compiler.Code.compile` gives an array with the `Compiler.NextOfLt` and `NFA.Capture.valid` property
+
+- `c_compile_spec`: main result
+-/
+
+open Std.Do
+
+set_option mvcgen.warning false
+
+@[spec] theorem c_bounded.fold.patch.pre_spec (compiled: ThompsonRef) (prev_end : Unchecked.StateID)
+  (greedy : Bool) (states : Array Unchecked.State)
+    : ⦃fun s => ⌜s = states ∧ tRefLt compiled states
+                      ∧ prev_end < states.size ∧ NextOfLt states
+                      ∧ patchAssignable states prev_end⌝⦄
+      Code.c_bounded.fold.patch.pre compiled prev_end greedy
+      ⦃post⟨fun r s => ⌜stateIdNextOfLt states r s ∧ assignableIf states s ∧ patchAssignable s r⌝, fun _ => ⌜False⌝⟩⦄ := by
+  mvcgen [Code.c_bounded.fold.patch.pre] with grind
+  and_intros
+  all_goals grind
+
+@[spec] theorem c_bounded.fold.patch.possessive_spec (compiled: ThompsonRef) (empty : Unchecked.StateID)
+  (states : Array Unchecked.State)
+    : ⦃fun s => ⌜s = states ∧ tRefLt compiled states
+                      ∧ empty < states.size ∧ NextOfLt states ∧ patchAssignable states compiled.end⌝⦄
+      Code.c_bounded.fold.patch.possessive compiled empty
+      ⦃post⟨fun r s => ⌜stateIdNextOfLeLt states r s ∧ assignableIf states s ∧ patchAssignable s r⌝, fun _ => ⌜False⌝⟩⦄ := by
+  mvcgen [Code.c_bounded.fold.patch.possessive] with grind
+
+@[spec] theorem c_bounded.fold.patch.post_spec (compiled: ThompsonRef) (union empty : Unchecked.StateID) (states : Array Unchecked.State)
+    : ⦃fun s => ⌜s = states ∧ compiled.end < states.size
+                      ∧ union < states.size ∧ empty < states.size ∧ NextOfLt states
+                      ∧ patchAssignable states union ∧ patchAssignable states compiled.end⌝⦄
+      Code.c_bounded.fold.patch.post compiled union empty
+      ⦃post⟨fun r s => ⌜stateIdNextOfLeLt states r s ∧ assignableIf states s ∧ patchAssignable s r⌝, fun _ => ⌜False⌝⟩⦄ := by
+  mvcgen [Code.c_bounded.fold.patch.post] with grind
+
+@[spec] theorem c_bounded.fold.patch_spec (compiled: ThompsonRef) (prev_end empty : Unchecked.StateID)
+  (greedy : Bool) (possessive : Bool) (states : Array Unchecked.State)
+    : ⦃fun s => ⌜s = states ∧ tRefLt compiled states
+                      ∧ prev_end < states.size ∧ empty < states.size ∧ NextOfLt states
+                      ∧ patchAssignable states prev_end ∧ patchAssignable states compiled.end⌝⦄
+      Code.c_bounded.fold.patch compiled prev_end empty greedy possessive
+      ⦃post⟨fun r s => ⌜stateIdNextOfLt states r s ∧ assignableIf states s ∧ patchAssignable s r⌝, fun _ => ⌜False⌝⟩⦄ := by
+  mvcgen [Code.c_bounded.fold.patch] with grind
+
+@[spec] theorem c_bounded.fold.patch_lift_spec  (compiled: ThompsonRef) (prev_end empty : Unchecked.StateID)
+  (greedy : Bool) (possessive : Bool) (states : Array Unchecked.State) (captures : Array NFA.Capture)
+    : ⦃fun s => ⌜(s.1 = states ∧ tRefLt compiled states
+                      ∧ prev_end < states.size ∧ empty < states.size ∧ NextOfLt states
+                      ∧ patchAssignable states prev_end ∧ patchAssignable states compiled.end)
+                  ∧ s.2.1 = captures ∧ cValid captures⌝⦄
+      (Code.c_bounded.fold.patch compiled prev_end empty greedy possessive : Code.CompilerM Unchecked.StateID)
+      ⦃post⟨fun r s => ⌜(stateIdNextOfLt states r s.1 ∧ assignableIf states s.1 ∧ patchAssignable s.1 r) ∧ s.2.1 = captures ∧ cMemAndValid captures s.2.1⌝, fun _ => ⌜False⌝⟩⦄ := by
+  exact coe_spec_EStateM_to_CompilerM (c_bounded.fold.patch_spec _ _ _ _ _ _)
+
+@[spec] theorem c_alt_iter_step_spec (first second: ThompsonRef) (states : Array Unchecked.State)
+    : ⦃fun s => ⌜s = states ∧ tRefLt first states
+                      ∧ tRefLt second states ∧ NextOfLt states
+                      ∧ patchAssignable states first.end ∧ patchAssignable states second.end⌝⦄
+      Code.c_alt_iter_step first second
+      ⦃post⟨fun r s => ⌜tRefNextOfLt states ⟨r.1, r.2⟩ s ∧ assignableIf states s ∧ patchAssignable s r.1 ∧ patchAssignable s r.2⌝, fun _ => ⌜False⌝⟩⦄ := by
+  mvcgen [Code.c_alt_iter_step] with grind
+
+@[spec] theorem c_alt_iter_step_lift_spec (first second: ThompsonRef) (states : Array Unchecked.State)
+  (captures : Array NFA.Capture)
+    : ⦃fun s => ⌜(s.1 = states ∧ tRefLt first states ∧ tRefLt second states ∧ NextOfLt states
+                    ∧ patchAssignable states first.end ∧ patchAssignable states second.end)
+                ∧ s.2.1 = captures ∧ cValid captures⌝⦄
+      (Code.c_alt_iter_step first second : Code.CompilerM (Unchecked.StateID × Unchecked.StateID))
+      ⦃post⟨fun r s => ⌜(tRefNextOfLt states ⟨r.1, r.2⟩ s.1 ∧ assignableIf states s.1 ∧ patchAssignable s.1 r.1 ∧ patchAssignable s.1 r.2)
+                        ∧ s.2.1 = captures ∧ cMemAndValid captures s.2.1⌝, fun _ => ⌜False⌝⟩⦄ := by
+  exact coe_spec_EStateM_to_CompilerM (c_alt_iter_step_spec _ _ _)
+
+@[spec] theorem c_rep_pre_spec (greedy : Bool) (states : Array Unchecked.State)
+    : ⦃fun s => ⌜s = states ∧ NextOfLt states⌝⦄
+      Code.c_rep_pre greedy
+      ⦃post⟨fun r s => ⌜stateIdNextOfLt states r s ∧ assignableIf states s ∧ patchAssignable s r⌝, fun _ => ⌜False⌝⟩⦄ := by
+  mintro _
+  dsimp [Code.c_rep_pre]
+  intros
+  mspec greedy_union_spec
+
+@[spec] theorem c_rep_pre_lift_spec (greedy : Bool) (states : Array Unchecked.State)
+  (captures : Array NFA.Capture)
+    : ⦃fun s => ⌜(s.1 = states ∧ NextOfLt states) ∧ s.2.1 = captures ∧ cValid captures⌝⦄
+      (Code.c_rep_pre greedy : Code.CompilerM Unchecked.StateID)
+      ⦃post⟨fun r s => ⌜(stateIdNextOfLt states r s.1 ∧ assignableIf states s.1 ∧ patchAssignable s.1 r) ∧ s.2.1 = captures ∧ cMemAndValid captures s.2.1⌝, fun _ => ⌜False⌝⟩⦄ := by
+  exact coe_spec_EStateM_to_CompilerM (c_rep_pre_spec _ _)
+
+set_option maxHeartbeats 4000000
+
+mutual
+
+@[spec] theorem c_alt_iter_fold_spec (hirs : Array Hir) (union «end» : Unchecked.StateID)
+  (states : Array Unchecked.State) (captures : Array NFA.Capture)
+    : ⦃fun s => ⌜s.1 = states ∧ union < states.size ∧ «end» < states.size ∧ NextOfLt states
+                ∧ patchAssignable states union
+                ∧ s.2.1 = captures ∧ cValid captures⌝⦄
+      Code.c_alt_iter.fold hirs union «end»
+      ⦃post⟨fun _ s => ⌜statesNextOfLeLt states s.1 ∧ assignableIf states s.1 ∧ cMemAndValid captures s.2.1⌝, fun _ => ⌜False⌝⟩⦄ := by
+  mintro _
+  unfold Code.c_alt_iter.fold
+  mspec Spec.foldlM_array
+  case inv =>
+    exact (fun (_, xs) s => ⌜states.size ≤ s.1.size ∧ union < s.1.size ∧ «end» < s.1.size
+                              ∧ assignableIf states s.1 ∧ patchAssignable states union
+                              ∧ NextOfLt s.1 ∧ cMemAndValid captures s.2.1⌝, fun e => ⌜False⌝, ())
+  case step =>
+    intros
+    expose_names
+    have := Array.sizeOf_lt_of_mem cur.property
+    mintro _
+    mspec c_spec
+    inst_mvars
+    case post.success =>
+      mspec patch_lift_spec
+      inst_mvars
+      case post.success =>
+        mspec patch_lift_spec
+        inst_mvars
+        case post.success =>
+          mvcgen with grind [= cMemAndValid]
+        all_goals grind [= cMemAndValid]
+      all_goals grind [= cMemAndValid]
+    all_goals grind
+  case pre =>
+    simp_all
+  case post =>
+    simp
+    all_goals grind [= cMemAndValid]
+  simp
+termination_by sizeOf hirs
+
+@[spec] theorem c_concat_fold_spec (tail : Array Hir) (sid : Unchecked.StateID)
+ (states : Array Unchecked.State) (captures : Array NFA.Capture)
+    : ⦃fun s => ⌜(s.1 = states ∧ sid < states.size ∧ NextOfLt states ∧ patchAssignable states sid) ∧ s.2.1 = captures ∧ cValid captures⌝⦄
+      Code.c_concat.fold tail sid
+      ⦃post⟨fun r s => ⌜stateIdNextOfLeLt states r s.1 ∧ assignableIf states s.1 ∧ patchAssignable s.1 r ∧ cMemAndValid captures s.2.1⌝, fun _ => ⌜False⌝⟩⦄ := by
+  mintro _
+  unfold Code.c_concat.fold
+  mspec Spec.foldlM_array
+  case inv =>
+    exact (fun (xs, r) s => ⌜states.size ≤ s.1.size ∧ sid < s.1.size ∧ r < s.1.size ∧ NextOfLt s.1
+                              ∧ assignableIf states s.1 ∧ patchAssignable s.1 r
+                              ∧ cMemAndValid captures s.2.1⌝, fun e => ⌜False⌝, ())
+  case pre => simp_all
+  case step =>
+    intros
+    expose_names
+    have := Array.sizeOf_lt_of_mem cur.property
+    mintro _
+    mspec c_spec
+    inst_mvars
+    case post.success =>
+      mspec patch_lift_spec
+      · inst_mvars
+        all_goals grind [= cMemAndValid]
+      · mvcgen
+        grind [= cMemAndValid]
+    all_goals grind
+  simp
+  grind [= cMemAndValid]
+  simp
+termination_by sizeOf tail
+
+@[spec] theorem c_alt_iter_spec (alt : Syntax.Alternation) (states : Array Unchecked.State)
+  (captures : Array NFA.Capture)
+    : ⦃fun s => ⌜s.1 = states ∧  NextOfLt states ∧ s.2.1 = captures ∧ cValid captures⌝⦄
+      Code.c_alt_iter alt
+      ⦃post⟨fun r s => ⌜tRefNextOfLt states r s.1 ∧ assignableIf states s.1 ∧ patchAssignable s.1 r.end ∧ cMemAndValid captures s.2.1⌝, fun _ => ⌜False⌝⟩⦄ := by
+  mintro _
+  unfold Code.c_alt_iter
+  split
+  expose_names
+  have : sizeOf first < sizeOf (Syntax.Alternation.mk first second tail) := by simp +arith
+  have : sizeOf second < sizeOf (Syntax.Alternation.mk first second tail) := by simp +arith
+  have : sizeOf tail < sizeOf (Syntax.Alternation.mk first second tail) := by simp +arith
+  mspec c_spec
+  inst_mvars; grind; grind
+  mspec c_spec
+  inst_mvars
+  case post.success.post.success =>
+    mspec c_alt_iter_step_lift_spec
+    inst_mvars
+    case post.success =>
+      mspec c_alt_iter_fold_spec
+      inst_mvars
+      case post.success =>
+        mvcgen with grind [= cMemAndValid]
+      all_goals grind
+    all_goals grind
+  all_goals grind
+termination_by sizeOf alt
+
+@[spec] theorem c_bounded_spec (hir : Hir) (min max : Nat) (greedy : Bool) (possessive : Bool)
+  (states : Array Unchecked.State) (captures : Array NFA.Capture)
+    : ⦃fun s => ⌜s.1 = states ∧  NextOfLt states ∧ s.2.1 = captures ∧ cValid captures⌝⦄
+      Code.c_bounded hir min max greedy possessive
+      ⦃post⟨fun r s => ⌜tRefNextOfLt states r s.1 ∧ assignableIf states s.1 ∧ patchAssignable s.1 r.end ∧ cMemAndValid captures s.2.1⌝, fun _ => ⌜False⌝⟩⦄ := by
+  mintro _
+  unfold Code.c_bounded
+  split
+  mspec c_exactly_spec
+  inst_mvars; grind; grind
+  split
+  case isTrue.post.success.isTrue =>
+    split
+    · mspec c_possessive_le_lift_spec
+      inst_mvars
+      case post.success => mvcgen with grind
+      all_goals grind
+    · simp
+      intros
+      and_intros
+      all_goals grind [= cMemAndValid]
+  case isTrue.post.success.isFalse =>
+      mspec add_empty_lift_spec'
+      inst_mvars
+      case post.success =>
+        mspec c_bounded_fold_spec
+        inst_mvars
+        case post.success =>
+          mspec patch_lift_spec
+          · inst_mvars; all_goals grind
+          · simp
+            all_goals grind [= cMemAndValid]
+        all_goals grind
+      all_goals grind
+  case isFalse =>
+    mspec c_empty_lift_spec
+    inst_mvars
+    case post.success => mvcgen with grind
+    all_goals grind
+termination_by sizeOf hir + sizeOf min + sizeOf (max - min) + 1
+
+@[spec] theorem c_lookaround_spec (look : Lookaround) (states : Array Unchecked.State)
+  (captures : Array NFA.Capture)
+    : ⦃fun s => ⌜s.1 = states ∧ NextOfLt states ∧ s.2.1 = captures ∧ cValid captures⌝⦄
+      Code.c_lookaround look
+      ⦃post⟨fun r s => ⌜tRefNextOfLt states r s.1 ∧ assignableIf states s.1 ∧ patchAssignable s.1 r.end ∧ cMemAndValid captures s.2.1⌝, fun _ => ⌜False⌝⟩⦄ := by
+  mintro _
+  unfold Code.c_lookaround
+  split
+  case h_1 | h_2 =>
+    mspec c_spec
+    inst_mvars; grind; grind
+    mspec
+    inst_mvars; grind; grind; grind; grind; grind
+    simp
+    all_goals grind [= cMemAndValid]
+  case h_3 | h_4 =>
+    mspec add_next_char_lift_spec
+    inst_mvars
+    case post.success =>
+      mspec c_spec
+      inst_mvars
+      case post.success =>
+        mspec
+        inst_mvars
+        case post.success => simp; intros; grind
+        all_goals simp_all
+        all_goals grind
+      all_goals grind
+    all_goals grind
+termination_by sizeOf look
+
+@[spec] theorem c_repetition_spec (rep : Repetition) (states : Array Unchecked.State)
+  (captures : Array NFA.Capture)
+    : ⦃fun s => ⌜s.1 = states ∧ NextOfLt states ∧ s.2.1 = captures ∧ cValid captures⌝⦄
+      Code.c_repetition rep
+      ⦃post⟨fun r s => ⌜tRefNextOfLt states r s.1 ∧ assignableIf states s.1 ∧ patchAssignable s.1 r.end ∧ cMemAndValid captures s.2.1⌝, fun _ => ⌜False⌝⟩⦄ := by
+  mintro _
+  unfold Code.c_repetition
+  split
+  case h_1 | h_2 =>
+    mspec
+    inst_mvars
+    case post.success =>
+      mspec c_spec
+      inst_mvars
+      case post.success =>
+        mspec
+        inst_mvars
+        case post.success => mvcgen with grind
+        all_goals grind
+      all_goals grind
+    all_goals grind
+  case h_3 =>
+    split
+    · mspec
+      inst_mvars
+      case post.success =>
+        mspec c_spec
+        inst_mvars
+        case post.success =>
+          mspec
+          inst_mvars
+          case post.success => mvcgen with grind
+          all_goals grind
+        all_goals grind
+      all_goals grind
+    · mspec c_at_least_spec
+  case h_4 =>
+    split
+    mspec c_bounded_spec
+    mspec c_empty_lift_spec
+    inst_mvars; grind; grind
+    simp
+    intros
+    grind [= cMemAndValid]
+termination_by sizeOf rep
+
+@[spec] theorem c_exactly_spec (hir : Hir) (n : Nat) (states : Array Unchecked.State)
+   (captures : Array NFA.Capture)
+    : ⦃fun s => ⌜s.1 = states ∧  NextOfLt states ∧ s.2.1 = captures ∧ cValid captures⌝⦄
+      Code.c_exactly hir n
+      ⦃post⟨fun r s => ⌜tRefNextOfLt states r s.1 ∧ assignableIf states s.1 ∧ patchAssignable s.1 r.end ∧ cMemAndValid captures s.2.1⌝, fun _ => ⌜False⌝⟩⦄ := by
+  mintro _
+  unfold Code.c_exactly
+  split
+  · mspec c_spec
+    inst_mvars; grind; grind
+    mspec c_exactly_fold_spec
+    inst_mvars
+    case isTrue.post.success.post.success => mvcgen with grind [= cValid, = cMemAndValid]
+    all_goals grind
+  · mspec c_empty_lift_spec
+    inst_mvars
+    case isFalse.post.success => mvcgen with grind
+    all_goals grind
+termination_by sizeOf hir + sizeOf n
+
+@[spec] theorem c_concat_spec (hirs : Array Hir) (states : Array Unchecked.State) (captures : Array NFA.Capture)
+    : ⦃fun s => ⌜(s.1 = states ∧ NextOfLt states) ∧ s.2.1 = captures ∧ cValid captures⌝⦄
+      Code.c_concat hirs
+      ⦃post⟨fun r s => ⌜tRefNextOfLt states r s.1 ∧ assignableIf states s.1 ∧ patchAssignable s.1 r.end ∧ cMemAndValid captures s.2.1⌝, fun _ => ⌜False⌝⟩⦄ := by
+  mintro _
+  unfold Code.c_concat
+  split
+  expose_names
+  have := Array.sizeOf_head?_of_mem heq
+  have := Array.sizeOf_head?_of_tail heq
+  mspec c_spec
+  inst_mvars
+  case h_1.post.success =>
+    mspec c_concat_fold_spec
+    inst_mvars
+    case post.success =>
+      mvcgen with grind [= cValid, = cMemAndValid]
+    all_goals grind
+  case h_2 =>
+    mvcgen
+    inst_mvars
+    all_goals grind [= cValid, = cMemAndValid]
+  all_goals grind
+termination_by sizeOf hirs
+
+@[spec] theorem c_exactly_fold_spec (hir : Hir) (n : Nat) («end» : Unchecked.StateID)
+  (states : Array Unchecked.State) (captures : Array NFA.Capture)
+    : ⦃fun s => ⌜s.1 = states ∧ «end» < states.size ∧  NextOfLt states
+                  ∧ patchAssignable states «end»
+                  ∧ s.2.1 = captures ∧ cValid captures⌝⦄
+      Code.c_exactly.fold hir n «end»
+      ⦃post⟨fun r s => ⌜stateIdNextOfLeLt states r s.1 ∧ assignableIf states s.1 ∧ patchAssignable s.1 r ∧ cMemAndValid captures s.2.1⌝, fun _ => ⌜False⌝⟩⦄ := by
+  mintro _
+  unfold Code.c_exactly.fold
+  split
+  mspec Spec.foldlM_list
+  case inv =>
+    exact (fun (xs, r) s => ⌜states.size ≤ s.1.size ∧ r < s.1.size ∧ «end» < s.1.size
+                              ∧ assignableIf states s.1 ∧ patchAssignable s.1 r ∧ patchAssignable states «end»
+                              ∧ NextOfLt s.1 ∧ cMemAndValid captures s.2.1⌝, fun e => ⌜False⌝, ())
+  case step =>
+    intros
+    mintro _
+    mspec c_spec
+    inst_mvars
+    case post.success =>
+      mspec patch_lift_spec
+      inst_mvars
+      case post.success => mvcgen with grind [= cMemAndValid]
+      all_goals grind [= cMemAndValid]
+    all_goals grind
+  case pre | isFalse =>
+    simp_all
+  case isTrue.post =>
+    simp
+    all_goals grind [= cMemAndValid]
+  simp
+termination_by sizeOf hir + sizeOf n
+
+@[spec] theorem c_at_least_spec (hir : Hir) (n : Nat) (greedy : Bool) (possessive : Bool)
+  (states : Array Unchecked.State) (captures : Array NFA.Capture)
+    : ⦃fun s => ⌜s.1 = states ∧  NextOfLt states ∧ s.2.1 = captures ∧ cValid captures⌝⦄
+      Code.c_at_least hir n greedy possessive
+      ⦃post⟨fun r s => ⌜tRefNextOfLt states r s.1 ∧ assignableIf states s.1 ∧ patchAssignable s.1 r.end ∧ cMemAndValid captures s.2.1⌝, fun _ => ⌜False⌝⟩⦄ := by
+  mintro _
+  unfold Code.c_at_least
+  split
+  case isTrue =>
+    mspec c_spec
+    inst_mvars; grind; grind
+    mspec c_at_least_0_spec
+    inst_mvars
+    case post.success.post.success =>
+      mspec c_at_least_0_post_lift_spec
+      inst_mvars
+      case post.success => mvcgen with grind
+      all_goals grind
+    all_goals grind
+  case isFalse =>
+    split
+    mspec c_spec
+    inst_mvars; grind; grind
+    mspec c_at_least_1_spec
+    inst_mvars
+    case isTrue.post.success.post.success =>
+      mspec c_at_least_1_post_lift_spec
+      inst_mvars
+      case post.success => simp; intros; grind [= cMemAndValid]
+      all_goals grind [= cMemAndValid]
+    case isFalse =>
+      mspec c_exactly_spec
+      inst_mvars; grind; grind
+      mspec c_spec
+      inst_mvars
+      case post.success.post.success =>
+        mspec c_at_least_2_lift_spec
+        inst_mvars
+        case post.success => simp; intros; grind [= cMemAndValid]
+        all_goals grind
+      all_goals grind
+    all_goals grind
+termination_by sizeOf hir + sizeOf n + 1
+
+@[spec] theorem c_bounded_fold_spec  (hir : Hir) (n : Nat) («prefix» : ThompsonRef) (empty : Unchecked.StateID)
+  (greedy : Bool) (possessive : Bool) (states : Array Unchecked.State) (captures : Array NFA.Capture)
+    : ⦃fun s => ⌜s.1 = states ∧ tRefLt «prefix» states ∧ empty < states.size ∧ NextOfLt states
+                 ∧ patchAssignable states «prefix».end
+                 ∧ s.2.1 = captures ∧ cValid captures⌝⦄
+      Code.c_bounded.fold hir n «prefix» empty greedy possessive
+      ⦃post⟨fun r s => ⌜stateIdNextOfLeLt states r s.1 ∧ assignableIf states s.1 ∧ patchAssignable s.1 r ∧ cMemAndValid captures s.2.1⌝, fun _ => ⌜False⌝⟩⦄ := by
+  mintro _
+  unfold Code.c_bounded.fold
+  split
+  mspec Spec.foldlM_list
+  case inv =>
+    exact (fun (xs, r) s => ⌜states.size ≤ s.1.size ∧ r < s.1.size ∧ empty < s.1.size
+                            ∧ assignableIf states s.1 ∧ patchAssignable s.1 r ∧ patchAssignable states «prefix».end
+                            ∧ NextOfLt s.1 ∧ cMemAndValid captures s.2.1⌝, fun e => ⌜False⌝, ())
+  case step =>
+    intros
+    mintro _
+    mspec c_spec
+    inst_mvars
+    case post.success =>
+      mspec c_bounded.fold.patch_lift_spec
+      inst_mvars
+      case post.success => mvcgen with grind [= cMemAndValid]
+      all_goals grind
+    all_goals grind
+  case pre =>
+    intro _
+    simp_all
+  case isTrue =>
+    simp
+    all_goals grind
+  case isFalse =>
+    intro _
+    simp_all
+  simp
+termination_by sizeOf hir + sizeOf n
+
+@[spec] theorem c_cap_spec (hir : Syntax.Capture) (states : Array Unchecked.State)
+  (captures : Array NFA.Capture)
+    : ⦃fun s => ⌜s.1 = states ∧  NextOfLt states ∧ s.2.1 = captures ∧ cValid captures⌝⦄
+      Code.c_cap hir
+      ⦃post⟨fun r s => ⌜tRefNextOfLt states r s.1 ∧ assignableIf states s.1 ∧ patchAssignable s.1 r.end ∧ cMemAndValid captures s.2.1⌝, fun _ => ⌜False⌝⟩⦄ := by
+  mintro _
+  unfold Code.c_cap
+  split
+  mspec c_cap'_start_spec
+  inst_mvars; grind; grind
+  mspec c_spec
+  inst_mvars
+  case h_1.post.success.post.success =>
+    intros
+    mspec c_cap'_end_spec
+    inst_mvars
+    case post.success =>
+      mspec patch_lift_spec
+      inst_mvars
+      case post.success =>
+        mspec patch_lift_spec
+        inst_mvars
+        case post.success =>
+          mvcgen with grind [= cMemAndValid]
+        all_goals grind
+      all_goals grind
+    simp_all
+    all_goals grind [= cMemAndValid]
+  all_goals grind
+termination_by sizeOf hir
+
+@[spec] theorem c_spec (hir : Hir) (states : Array Unchecked.State) (captures : Array NFA.Capture)
+    : ⦃fun s => ⌜s.1 = states ∧  NextOfLt states ∧ s.2.1 = captures ∧ cValid captures⌝⦄
+      Code.c hir
+      ⦃post⟨fun r s => ⌜tRefNextOfLt states r s.1 ∧ assignableIf states s.1 ∧ patchAssignable s.1 r.end ∧ cMemAndValid captures s.2.1⌝, fun _ => ⌜False⌝⟩⦄ := by
+  have : sizeOf hir.kind < sizeOf hir := Hir.sizeOfKindOfHir hir
+  mintro _
+  unfold Code.c
+  split
+  · mspec c_empty_lift_spec
+    inst_mvars; grind; grind; mvcgen with grind
+  · mspec c_literal_lift_spec
+    inst_mvars; grind; grind; mvcgen with grind
+  · mspec c_unicode_class_lift_spec
+    inst_mvars; grind; grind; mvcgen with grind
+  · mspec c_look_lift_spec
+    inst_mvars; grind; grind; mvcgen with grind
+  · expose_names
+    have : sizeOf look < sizeOf hir.kind := by simp [heq]
+    mspec c_lookaround_spec
+  · mspec c_back_ref_lift_spec
+    inst_mvars; grind; grind; mvcgen with grind
+  · expose_names
+    have : sizeOf rep < sizeOf hir.kind := by simp [heq]
+    mspec c_repetition_spec
+  · expose_names
+    have : sizeOf cap < sizeOf hir.kind := by simp [heq]
+    mspec c_cap_spec
+  · expose_names
+    have : sizeOf items < sizeOf hir.kind := by simp [heq]
+    mspec c_concat_spec
+    grind
+  · expose_names
+    have : sizeOf sub < sizeOf hir.kind := by simp [heq]
+    mspec c_alt_iter_spec
+termination_by sizeOf hir
+
+end
+
+@[spec] theorem c_init_spec (anchored : Bool)
+    : ⦃fun s => ⌜s.1.size = 0 ∧ s.2.1.size = 0⌝⦄
+      Code.init anchored
+      ⦃post⟨fun r s => ⌜tRefLt r s.1 ∧ NextOfLt s.1 ∧ patchAssignable s.1 r.end ∧ cValid s.2.1⌝, fun _ => ⌜False⌝⟩⦄ := by
+  mintro _
+  mvcgen [Code.init] with exact #[]
+  all_goals grind
+
+@[spec] theorem c_compile_spec (anchored : Bool) (hir : Hir)
+    : ⦃fun s => ⌜s.1.size = 0 ∧ s.2.1.size = 0⌝⦄
+      Code.compile anchored hir
+      ⦃post⟨fun _ s => ⌜NextOfLt s.1 ∧ cValid s.2.1⌝, fun _ => ⌜False⌝⟩⦄ := by
+  mintro _
+  unfold Code.compile
+  mspec c_init_spec
+  mspec c_cap_spec
+  inst_mvars
+  case success.post.success =>
+    mspec add_match_lift_spec
+    inst_mvars
+    case post.success =>
+      mspec patch_lift_spec
+      inst_mvars
+      case post.success =>
+        mvcgen
+        and_intros
+        simp
+        apply NextOfLt.mk
+        case vc1.pre.refine_2.refine_1 => rfl
+        all_goals grind
+      all_goals grind
+    all_goals grind
+  all_goals grind
+
+theorem compile_nextOf_lt {anchored : Bool} {expr : Hir}
+  (h : Code.compile anchored expr (#[], #[], #[]) = EStateM.Result.ok () (states, captures, groups))
+    : NextOfLt states := by
+  have heq := c_compile_spec anchored expr (#[], #[], #[])
+  simp [wp] at heq
+  split at heq <;> simp_all
+
+theorem compile_captures_valid {anchored : Bool} {expr : Hir}
+  (h : Code.compile anchored expr (#[], #[], #[]) = EStateM.Result.ok () (states, captures, groups))
+    : Capture.Valid captures := by
+  have heq := c_compile_spec anchored expr (#[], #[], #[])
+  simp [wp] at heq
+  split at heq <;> grind [= cValid]
+
+theorem compile_eq_ok {anchored : Bool} {expr : Hir}
+   : ∃ s, Code.compile anchored expr (#[], #[], #[]) = EStateM.Result.ok () s := by
+  have heq := c_compile_spec anchored expr (#[], #[], #[])
+  simp [wp] at heq
+  split at heq <;> simp_all
